galois/bitvec/rotate.lean
@@ -1,3 +1,4 @@
+import data.bitvec
 import galois.vector.rotate
 
 namespace bitvec
