galois/temporal/classical.lean
@@ -1,5 +1,4 @@
 import .temporal
-       init.classical
 
 universes u
 
