galois/vector/init_last.lean
@@ -1,5 +1,5 @@
 /- This defines init and last on vectors. -/
-import galois.list.init
+import ..list.init
 import .simplify_eq
 
 universe variables u
@@ -27,7 +27,7 @@ def init : vector α n → vector α (n-1)
 def last : vector α (nat.succ n) → α
 | ⟨l,p⟩ := list.last l (eq_succ_implies_non_nil p)
 
-theorem init_append_last_self {n : ℕ} (x : vector α (nat.succ n)) 
+theorem init_append_last_self {n : ℕ} (x : vector α (nat.succ n))
 : init x ++ vector.cons (last x) vector.nil = x :=
 begin
   cases x with v p,
